avx2 arithmetic propagate

libcrux-intrinsics/src/avx2_extract.rs
@@ -8,7 +8,9 @@
 #[hax_lib::fstar::replace(
     interface,
     "unfold type $:{Vec256} = bit_vec 256
-				      val vec256_as_i16x16 (x:t_Vec256) : t_Array i16 (sz 16)"
+     val vec256_as_i16x16 (x:t_Vec256) : t_Array i16 (sz 16)
+     let get_lane (v:t_Vec256) (i:nat{i < 16}) =
+       Seq.index (vec256_as_i16x16 v) i"
 )]
 pub struct Vec256(u8);
 
@@ -17,7 +19,9 @@ pub struct Vec256(u8);
 #[hax_lib::fstar::replace(
     interface,
     "unfold type $:{Vec128} = bit_vec 128
-				      val vec128_as_i16x8 (x:t_Vec128) : t_Array i16 (sz 8)"
+     val vec128_as_i16x8 (x:t_Vec128) : t_Array i16 (sz 8)
+     let get_lane128 (v:t_Vec128) (i:nat{i < 8}) =
+       Seq.index (vec128_as_i16x8 v) i"
 )]
 pub struct Vec128(u8);
 
